backends/lean/Aeneas/Tactic/Step/Tests.lean
@@ -8,3 +8,4 @@ import Aeneas.Tactic.Step.Tests.SpecParameters
 import Aeneas.Tactic.Step.Tests.TupleDestruct
 import Aeneas.Tactic.Step.Tests.UncurryBind
 import Aeneas.Tactic.Step.Tests.IntroTactic
+import Aeneas.Tactic.Step.Tests.IntroRecursion
